LeanSubst/Class.lean
@@ -20,22 +20,22 @@ theorem Ren.apply_id1 [RenMap S [T]] [RenMapId S [T]] {s : S} : s⟨id T⟩ = s 
 theorem Ren.apply_id2 [RenMap S [T1, T2]] [RenMapId S [T1, T2]] {s : S} : s⟨id T1, id T2⟩ = s := RenMapId.apply_id
 
 class RenMapCompose (S : Type u1) (V : List (Type u2)) [RenMap S V] where
-  apply_compose {s : S} {r1 r2 : List.Tuple Ren V} : s⟨r1,⟩⟨r2,⟩ = s⟨r1 ∘ r2,⟩
+  apply_compose {s : S} {r1 r2 : List.Tuple Ren V} : s⟨r1,⟩⟨r2,⟩ = s⟨r1 >> r2,⟩
 
 @[simp, grind =]
 theorem Ren.apply_compose [RenMap S V] [RenMapCompose S V] {s : S} {r1 r2 : List.Tuple Ren V}
-  : s⟨r1,⟩⟨r2,⟩ = s⟨r1 ∘ r2,⟩
+  : s⟨r1,⟩⟨r2,⟩ = s⟨r1 >> r2,⟩
 := RenMapCompose.apply_compose
 
 @[simp, grind =]
 theorem Ren.apply_compose1 [RenMap S [T]] [RenMapCompose S [T]] {s : S} {r1 r2 : Ren T}
-  : s⟨r1⟩⟨r2⟩ = s⟨r1 ∘ r2⟩
+  : s⟨r1⟩⟨r2⟩ = s⟨r1 >> r2⟩
 := Ren.apply_compose
 
 @[simp, grind =]
 theorem Ren.apply_compose2 [RenMap S [T1, T2]] [RenMapCompose S [T1, T2]]
   {s : S} {r1 r2 : Ren T1} {k1 k2 : Ren T2}
-  : s⟨r1, k1⟩⟨r2, k2⟩ = s⟨r1 ∘ r2, k1 ∘ k2⟩
+  : s⟨r1, k1⟩⟨r2, k2⟩ = s⟨r1 >> r2, k1 >> k2⟩
 := Ren.apply_compose
 
 instance (priority := high) [RenMap T [T]] [RenMapId T [T]] : RenMapId (Action T) [T] where
@@ -49,7 +49,7 @@ instance (priority := high) [RenMap T [T]] [RenMapCompose T [T]] : RenMapCompose
     intro s r1 r2; cases s
     all_goals
       simp [List.Tuple] at r1 r2
-      simp [rmap, Ren.compose_tuple]
+      simp [rmap, HAndThen.hAndThen, AndThen.andThen, Ren.compose_tuple, Ren.compose]
 
 instance (priority := low) [RenMap S V] [RenMapCompose S V] : RenMapCompose (Action S) V where
   apply_compose := by intro s; cases s <;> simp
@@ -70,81 +70,81 @@ theorem Subst.apply_id1 [SubstMap S [T]] [SubstMapId S [T]] {s : S} : s[id T] = 
 theorem Subst.apply_id2 [SubstMap S [T1, T2]] [SubstMapId S [T1, T2]] {s : S} : s[id T1, id T2] = s := SubstMapId.apply_id
 
 class SubstMapRenComposeLeft (S : Type u1) (V : List $ Type u2) [RenMap S V] [SubstMap S V] where
-  apply_ren_compose_left {s : S} {r : List.Tuple Ren V} {τ : List.Tuple Subst V} : s⟨r,⟩[τ,] = s[r ∘ τ,]
+  apply_ren_compose_left {s : S} {r : List.Tuple Ren V} {τ : List.Tuple Subst V} : s⟨r,⟩[τ,] = s[r >> τ,]
 
 @[simp, grind =]
 theorem Subst.apply_ren_compose_left
   [RenMap S V] [SubstMap S V] [SubstMapRenComposeLeft S V]
   {s : S} {r : List.Tuple Ren V} {σ : List.Tuple Subst V}
-  : s⟨r,⟩[σ,] = s[r ∘ σ,]
+  : s⟨r,⟩[σ,] = s[r >> σ,]
 := SubstMapRenComposeLeft.apply_ren_compose_left
 
 @[simp, grind =]
 theorem Subst.apply_ren_compose_left1
   [RenMap S [T]] [SubstMap S [T]] [SubstMapRenComposeLeft S [T]]
   {s : S} {r : Ren T} {σ : Subst T}
-  : s⟨r⟩[σ] = s[r ∘ σ]
+  : s⟨r⟩[σ] = s[r >> σ]
 := Subst.apply_ren_compose_left
 
 @[simp, grind =]
 theorem Subst.apply_ren_compose_left2
   [RenMap S [T1, T2]] [SubstMap S [T1, T2]] [SubstMapRenComposeLeft S [T1, T2]]
   {s : S} {r1 : Ren T1} {r2 : Ren T2} {σ1 : Subst T1} {σ2 : Subst T2}
-  : s⟨r1, r2⟩[σ1, σ2] = s[r1 ∘ σ1, r2 ∘ σ2]
+  : s⟨r1, r2⟩[σ1, σ2] = s[r1 >> σ1, r2 >> σ2]
 := Subst.apply_ren_compose_left
 
 class SubstMapRenComposeRight (S : Type u1) (V : List $ Type u2) [RenMap S V] [RenMapAll V] [SubstMap S V] where
-  apply_ren_compose_right {s : S} {r : List.Tuple Ren V} {σ : List.Tuple Subst V} : s[σ,]⟨r,⟩ = s[σ ∘ r,]
+  apply_ren_compose_right {s : S} {r : List.Tuple Ren V} {σ : List.Tuple Subst V} : s[σ,]⟨r,⟩ = s[σ >> r,]
 
 @[simp, grind =]
 theorem Subst.apply_ren_compose_right
   [RenMap S V] [RenMapAll V] [SubstMap S V] [SubstMapRenComposeRight S V]
   {s : S} {r : List.Tuple Ren V} {σ : List.Tuple Subst V}
-  : s[σ,]⟨r,⟩ = s[σ ∘ r,]
+  : s[σ,]⟨r,⟩ = s[σ >> r,]
 := SubstMapRenComposeRight.apply_ren_compose_right
 
 @[simp, grind =]
 theorem Subst.apply_ren_compose_right1
   [RenMap S [T]] [RenMapAll [T]] [SubstMap S [T]] [SubstMapRenComposeRight S [T]]
   {s : S} {r : Ren T} {σ : Subst T}
-  : s[σ]⟨r⟩ = s[σ ∘ r]
+  : s[σ]⟨r⟩ = s[σ >> r]
 := Subst.apply_ren_compose_right
 
 @[simp, grind =]
 theorem Subst.apply_ren_compose_right2
   [RenMap S [T1, T2]] [RenMapAll [T1, T2]] [SubstMap S [T1, T2]] [SubstMapRenComposeRight S [T1, T2]]
   {s : S} {r1 : Ren T1} {r2 : Ren T2} {σ1 : Subst T1} {σ2 : Subst T2}
-  : s[σ1, σ2]⟨r1, r2⟩ = s[σ1 ∘ r1, σ2 ∘ r2]
+  : s[σ1, σ2]⟨r1, r2⟩ = s[σ1 >> r1, σ2 >> r2]
 := Subst.apply_ren_compose_right
 
 class SubstMapCompose (S : Type u1) (V : List $ Type u2) [SubstMap S V] [SubstMapAll V] where
-  apply_compose {s : S} {σ τ : List.Tuple Subst V} : s[σ,][τ,] = s[σ ∘ τ,]
+  apply_compose {s : S} {σ τ : List.Tuple Subst V} : s[σ,][τ,] = s[σ >> τ,]
 
 @[simp, grind =]
 theorem Subst.apply_compose
   [SubstMap S V] [SubstMapAll V] [SubstMapCompose S V]
   {s : S} {σ1 σ2 : List.Tuple Subst V}
-  : s[σ1,][σ2,] = s[σ1 ∘ σ2,]
+  : s[σ1,][σ2,] = s[σ1 >> σ2,]
 := SubstMapCompose.apply_compose
 
 @[simp, grind =]
 theorem Subst.apply_compose1
   [SubstMap S [T]] [SubstMap T [T]] [SubstMapCompose S [T]]
   {s : S} {σ1 σ2 : Subst T}
-  : s[σ1][σ2] = s[σ1 ∘ σ2]
+  : s[σ1][σ2] = s[σ1 >> σ2]
 := Subst.apply_compose
 
 @[simp, grind =]
 theorem Subst.apply_compose2
   [SubstMap S [T1, T2]] [SubstMap T1 [T1]] [SubstMap T2 [T2]] [SubstMapCompose S [T1, T2]]
   {s : S} {σ1 σ2 : Subst T1} {τ1 τ2 : Subst T2}
-  : s[σ1, τ1][σ2, τ2] = s[σ1 ∘ σ2, τ1 ∘ τ2]
+  : s[σ1, τ1][σ2, τ2] = s[σ1 >> σ2, τ1 >> τ2]
 := Subst.apply_compose
 
 -- @[simp↓, grind =]
 -- theorem Subst.apply_compose2 [SubstMap S [T1, T2]] [SubstMapCompose S [T1, T2]]
 --   {s : S} {r1 r2 : Subst T1} {k1 k2 : Subst T2}
---   : s⟨r1, k1⟩⟨r2, k2⟩ = s⟨r1 ∘ r2, k1 ∘ k2⟩
+--   : s⟨r1, k1⟩⟨r2, k2⟩ = s⟨r1 >> r2, k1 >> k2⟩
 -- := by
 --   have lem := @SubstMapCompose.apply_compose S [T1, T2] _ _ s (r1, k1, .up .unit) (r2, k2, .up .unit)
 --   rw [lem]; simp [Subst.compose_tuple]
@@ -171,14 +171,14 @@ theorem Subst.apply_compose2
 -- @[simp, grind =]
 -- theorem Subst.apply_ren_compose_left [RenMap S T] [SubstMap S T] [SubstMapRenComposeLeft S T]
 --   {s : S} {r : Ren T} {τ : Subst T}
---   : s⟨r⟩[τ] = s[r ∘ τ]
+--   : s⟨r⟩[τ] = s[r >> τ]
 -- := SubstMapRenComposeLeft.apply_ren_compose_left
 
 -- @[simp, grind =]
 -- theorem Subst.apply_ren_compose_right
 --   [RenMap S T] [RenMap T T] [SubstMap S T] [SubstMapRenComposeRight S T]
 --   {s : S} {σ : Subst T} {r : Ren T}
---   : s[σ]⟨r⟩ = s[σ ∘ r]
+--   : s[σ]⟨r⟩ = s[σ >> r]
 -- := SubstMapRenComposeRight.apply_ren_compose_right
 
 -- @[grind =]
@@ -198,7 +198,7 @@ theorem Subst.apply_compose2
 -- @[simp, grind =]
 -- theorem Subst.apply_compose [SubstMap S T] [SubstMap T T] [SubstMapCompose S T]
 --   {s : S} {σ τ : Subst T}
---   : s[σ][τ] = s[σ ∘ τ]
+--   : s[σ][τ] = s[σ >> τ]
 -- := SubstMapCompose.apply_compose
 
 -- @[simp, grind =]
